coq_general_theory/evolution_aware_instantiation.v
@@ -1,0 +1,162 @@
+Load model_evolution.
+
+Fixpoint findADD (key : string) (l : list (string * (ADD float)))
+  (default : ADD float) : ADD float :=
+  match l with
+  | nil => default
+  | (s , a) :: l' => if s =? key then a else findADD key l' default
+  end. 
+
+Fixpoint func_familyOperation (re : RatExpr)
+  (l : list (string * (ADD float))) : ADD float :=
+  match re with
+  | Const f => constant f
+  | OneVar v => findADD v l (constant 1%float)
+  | Sum r1 r2 => plus_add
+      (func_familyOperation r1 l)
+      (func_familyOperation r2 l)
+  | Sub r1 r2 => sub_add
+      (func_familyOperation r1 l)
+      (func_familyOperation r2 l)
+  | Mul r1 r2 => mult_add
+      (func_familyOperation r1 l)
+      (func_familyOperation r2 l)
+  | Div r1 r2 => div_add
+      (func_familyOperation r1 l)
+      (func_familyOperation r2 l)
+  | Minus r => opp_add
+      (func_familyOperation r l)
+  end.
+
+Instance PC_Rat_Expr : Asset (string * RatExpr) := 
+{
+  familyOperation := 
+    (fun ( p : string * RatExpr) (l : list (string * (ADD float))) =>
+    ((fst p) , func_familyOperation (snd p) l))
+}.
+
+Definition func_featureOperation (r : RDG) : (string * RatExpr) :=
+  match r with
+  | RDG_leaf s p => (s , snd p)
+  | RDG_cons s p l => (s , snd p)
+  end.
+
+Fixpoint RemoveVarExpr (s : string) (r : RatExpr) :=
+  match r with
+  | Const t => Const t
+  | OneVar s' => if s' =? s then Const 1.0 else OneVar s'
+  | Sum r1 r2 => Sum (RemoveVarExpr s r1) (RemoveVarExpr s r2)
+  | Sub r1 r2 => Sub (RemoveVarExpr s r1) (RemoveVarExpr s r2)
+  | Mul r1 r2 => Mul (RemoveVarExpr s r1) (RemoveVarExpr s r2)
+  | Div r1 r2 => Div (RemoveVarExpr s r1) (RemoveVarExpr s r2)
+  | Minus r => Minus (RemoveVarExpr s r)
+  end.
+
+Definition nameRDG (r : RDG) : string :=
+  match r with
+  | RDG_leaf s _ => s
+  | RDG_cons s _ _ => s
+  end.
+
+Fixpoint Instance_EvolutionRDG (delta : RDG -> Evolution) (r : RDG) : RDG :=
+  match r with
+  | RDG_leaf s (pc , re) => match (delta r) with
+                            | ID => r
+                            | Message => RDG_leaf s (pc, Mul re (Const 0.9))
+                            | PC => RDG_leaf s ("True", re)
+                            | AddFeature => RDG_cons s (pc, Mul re (OneVar "AF"))
+                                              ((RDG_leaf "AF" ("PCaf", Const 0.445))::nil)
+                            | _ => r
+                            end
+  | RDG_cons s (pc , re) l => match (delta r) with
+                              | ID => r
+                              | Message => RDG_cons s (pc, Mul re (Const 0.9))
+                                  (map (Instance_EvolutionRDG delta) l)
+                              | PC => RDG_cons s ("True", re)
+                                  (map (Instance_EvolutionRDG delta) l)
+                              | AddFeature => RDG_cons s (pc, Mul re (OneVar "AF"))
+                                         ((RDG_leaf "AF" ("PCaf", Const 0.445))::
+                                          (map (Instance_EvolutionRDG delta) l))
+                              | SubsequentModelEvol => RDG_cons s (pc , re)
+                                    (map (Instance_EvolutionRDG delta) l)
+                              | RemoveFeature => match l with
+                                                 | nil => r
+                                                 | h :: t => RDG_cons s 
+                                                  (pc , RemoveVarExpr (nameRDG h) re)
+                                                  (map (Instance_EvolutionRDG delta) t)
+                                                 end
+                              end
+  end.
+
+Definition Instance_ADDdepsRmvCase (r : RDG) (delta : RDG -> Evolution)
+  (l : list (string * (ADD float))) : list (string * (ADD float)) :=
+  match l with
+  | nil => nil
+  | h :: t => t
+  end.
+
+Inductive InductiveModel : Type :=
+  | Mod (r : RDG).
+
+Axiom ID_deps_evolution : forall (r : RDG) (delta : RDG -> Evolution),
+  delta r = ID -> (forall (rdg : RDG), In rdg (deps r) -> delta rdg = ID).
+
+Theorem ID_Evolution_list : forall (delta : RDG -> Evolution) (l : list RDG),
+  (forall (rdg : RDG), In rdg l -> delta rdg = ID) -> l = map (Instance_EvolutionRDG delta) l.
+Proof.
+  intros. induction l. auto. simpl. assert (H' : delta a = ID).
+  apply H. left. reflexivity. assert (H'' : Instance_EvolutionRDG delta a = a).
+  destruct a;destruct ass; unfold Instance_EvolutionRDG; rewrite H';auto.
+  rewrite H''. assert (H''' : forall (r : RDG) (l1 l2 : list RDG),
+  l1 = l2 -> r :: l1 = r :: l2). intros. rewrite H0. reflexivity.
+  apply H'''. apply IHl. intros. apply H. right. auto.
+Qed.
+
+Program Instance InstanceModel : Model InductiveModel := 
+{
+  buildRDG := (fun m : InductiveModel => match m with
+                                         | Mod r => r
+                                         end);
+
+  featureOperation := func_featureOperation;
+
+  evolutionRDG := (fun (r : RDG) (d : RDG -> Evolution) =>
+      Instance_EvolutionRDG d r);
+
+  AddedRDG := (fun (r : RDG) (d : RDG -> Evolution) =>
+      (RDG_leaf "AF" ("PCaf", Const 0.445)));
+
+  ADDdepsRmvCase := Instance_ADDdepsRmvCase;
+}.
+
+{ Next Obligation.
+  destruct rdg;destruct ass;
+  simpl; rewrite H; simpl; exists (RDG_leaf "AF" ("PCaf", Const 0.44500000000000001)).
+  - exists nil. auto.
+  - exists (map (Instance_EvolutionRDG delta) deps0). auto.
+Qed. }
+
+{ Next Obligation.
+  destruct rdg; destruct ass; simpl; rewrite H; auto.
+Qed. }
+
+{ Next Obligation.
+  destruct rdg; destruct ass; simpl.
+  - destruct (delta (RDG_leaf s (s0, r))); try (auto).
+    assert (H': AddFeature = AddFeature). reflexivity. apply H in H'.
+    destruct H'.
+  - remember (delta (RDG_cons s (s0, r) deps0)) as delt.
+    destruct delt; try auto.
+    + symmetry in Heqdelt.
+      assert (H' : (forall (rdg : RDG),
+        In rdg (deps (RDG_cons s (s0, r) deps0)) -> delta rdg = ID)).
+      apply ID_deps_evolution. auto. apply ID_Evolution_list. auto.
+    + assert (H': AddFeature = AddFeature). reflexivity. apply H in H'.
+      destruct H'.
+    + assert (H': RemoveFeature = RemoveFeature). reflexivity. apply H0 in H'.
+      destruct H'.
+Qed. }
+
+
+
+
